\section{Derivatives of the potential}
\label{sec:pot_derivatives}

For completeness, we give here the full expression for the first few
derivatives of the potential that are used in our FMM scheme. We use
the notation $\mathbf{r}=(r_x, r_y, r_z)$, $r = |\mathbf{r}|$, $u=r/H$
and $x=2r/r_s$. We also assume $H \ll r_s$. We can construct the
higher order derivatives by successively applying the "chain rule". We
show representative examples of the first few relevant ones here split
by order. We start by constructing derivatives of the truncated
potentials. The first step is the construction of derivatives of the
long-range truncation function. We define
\begin{equation}
  \alpha(w) \equiv \left(1 + e^w\right)^{-1} \nonumber
\end{equation}
and compute its derivatives in terms of powers of $\alpha$ (note the
difference in notation between powers $\alpha^n$ and n-th derivatives
$\alpha^{(n)}$)\footnote{This can be computed by \textsc{Mathematica}
  using the expression \texttt{Apart[D[1/(1 + Exp[w]), {w, n}]]} for
  the n-th derivative.}:
\begin{align}
  \alpha^{(0)}(w) &= +\alpha(w), \nonumber\\
  \alpha^{(1)}(w) &= -\alpha(w) + \alpha^2(w),  \nonumber\\
  \alpha^{(2)}(w) &= +\alpha(w) - 3\alpha^2(w) + 2\alpha^3(w),  \nonumber\\
  \alpha^{(3)}(w) &= -\alpha(w) + 7\alpha^2(w) - 12\alpha^3(w) + 6\alpha^4(w),   \nonumber\\
  \alpha^{(4)}(w) &= +\alpha(w) - 15\alpha^2(w) + 50\alpha^3(w) - 60\alpha^4(w) + 24\alpha^5(w),    \nonumber\\
  \alpha^{(5)}(w) &= -\alpha(w) + 31\alpha^2(w) -180\alpha^3(w) + 390\alpha^4(w) -360\alpha^5(w) + 120\alpha^6(w).\nonumber                                      
\end{align}
We can then construct our sigmoid $\sigma(w) \equiv e^w\alpha(w)$ and
its derivatives, again in terms of powers of $\alpha(w)$ only:
\begin{align}
  \sigma^{(0)}(w) &= e^w\alpha(w), \nonumber\\
  \sigma^{(1)}(w) &= e^w\left(\alpha^{(1)}(w) + \alpha(w) \right) \nonumber\\
                  &= e^w \alpha^2(w), \nonumber \\
  \sigma^{(2)}(w) &= e^w\left(\alpha(w) +2\alpha^{(1)}(w) + \alpha^{(2)}(w)  \right) \nonumber\\
                  &= e^w \left(2\alpha^3(w) - \alpha^2(w)\right), \nonumber \\
  \sigma^{(3)}(w) &= e^w\left(\alpha(w) + 3\alpha^{(1)}(w) + 3\alpha^{(2)}(w) + \alpha^{(3)}(w)  \right) \nonumber\\
                  &= e^w \left(6\alpha^4(w) - 6\alpha^3(w) + \alpha^2(w)\right), \nonumber \\
  \sigma^{(4)}(w) &= e^w\left(\alpha(w) + 4\alpha^{(1)}(w) + 6\alpha^{(2)}(w) + 4\alpha^{(3)}(w) + \alpha^{(4)}(w)  \right) \nonumber\\
                  &= e^w \left(24\alpha^5(w) - 36\alpha^4(w) + 14\alpha^3(w) - \alpha^2(w)\right), \nonumber \\
  \sigma^{(5)}(w) &= e^w\left(\alpha(w) + 5\alpha^{(1)}(w) + 10\alpha^{(2)}(w) + 10\alpha^{(3)}(w) + 5\alpha^{(4)}(w) + \alpha^{(5)}(w)  \right) \nonumber\\
                  &= e^w \left(120\alpha^6(w) - 240\alpha^5(w) + 150\alpha^4(w) - 30\alpha^3(w) + \alpha^2(w)\right). \nonumber 
\end{align}
We can finally construct our long-range truncation function
$\chi(r,r_s) \equiv 2 - 2\sigma(2r/r_s)$ and its derivatives
\begin{align}
  \chi(r,r_s) &= 2 - 2e^{2r/r_s} \alpha(2r/r_s), \nonumber \\
  \frac{\partial}{\partial r} \chi(r, r_s) &= -2 \left(\frac{2}{r_s}\right)^1 \sigma^{(1)}\left(\frac{2r}{r_s}\right) = -2 \left(\frac{2}{r_s}\right)^1 e^{\frac{2r}{r_s}} \alpha^2 \left(\frac{2r}{r_s}\right), \nonumber\\
  \frac{\partial^2}{\partial r^2} \chi(r, r_s) &= -2 \left(\frac{2}{r_s}\right)^2 \sigma^{(2)}\left(\frac{2r}{r_s}\right) = -2 \left(\frac{2}{r_s}\right)^2  e^{\frac{2r}{r_s}} \left[2\alpha^3 \left(\frac{2r}{r_s}\right) - \alpha^2 \left(\frac{2r}{r_s}\right) \right], \nonumber\\
  \frac{\partial^3}{\partial r^3} \chi(r, r_s) &= -2 \left(\frac{2}{r_s}\right)^3 \sigma^{(3)}\left(\frac{2r}{r_s}\right) = -2 \left(\frac{2}{r_s}\right)^3  e^{\frac{2r}{r_s}} \left[6\alpha^4 \left(\frac{2r}{r_s}\right) - 6\alpha^3 \left(\frac{2r}{r_s}\right) + \alpha^2 \left(\frac{2r}{r_s}\right) \right],\nonumber \\
  \frac{\partial^4}{\partial r^4} \chi(r, r_s) &= -2 \left(\frac{2}{r_s}\right)^4 \sigma^{(4)}\left(\frac{2r}{r_s}\right) = -2 \left(\frac{2}{r_s}\right)^4  e^{\frac{2r}{r_s}} \left[24\alpha^5 \left(\frac{2r}{r_s}\right) - 36\alpha^4 \left(\frac{2r}{r_s}\right) + 14\alpha^3 \left(\frac{2r}{r_s}\right) - \alpha^2 \left(\frac{2r}{r_s}\right) \right],\nonumber \\
  \frac{\partial^5}{\partial r^5} \chi(r, r_s) &= -2 \left(\frac{2}{r_s}\right)^5 \sigma^{(5)}\left(\frac{2r}{r_s}\right) = -2 \left(\frac{2}{r_s}\right)^5  e^{\frac{2r}{r_s}} \left[120\alpha^6 \left(\frac{2r}{r_s}\right) - 240\alpha^5 \left(\frac{2r}{r_s}\right) + 150\alpha^4 \left(\frac{2r}{r_s}\right) - 30\alpha^3 \left(\frac{2r}{r_s}\right) + \alpha^2 \left(\frac{2r}{r_s}\right) \right].\nonumber
\end{align}
In the Newtonian limit ($r_s\rightarrow\infty$) the first expression
reduces to $\chi(r,r_s) = 1$ whilst all higher-order derivatives
vanish. In the limit $r\rightarrow\infty$ (and $r_s < \infty$), all terms vanish. All these
derivatives can be computed easily as they are simple polynomials of
$\alpha(2r/r_s)$. They involve one exponential and one inversion for
the initial calculation of $\alpha$ and all the other terms can be
obtained very eeficiently on modern architectures as they only involve
\emph{fused-multiple-add} operations.We can now construct common
quantities that appear in derivatives of multiple orders of the
truncated an softened gravity field $\varphi (\mathbf{r}, r_s, H)
\equiv \frac{1}{r}\chi(r,r_s)$:


% \begin{align}
%   \alpha(x) &= \left(1 + e^x\right)^{-1}  \nonumber \\
%   \chi(r, r_s) &= 2\left(1 - e^{2r/r_s}\alpha(2r/r_s) \right) \nonumber \\
%   \chi'(r, r_s) &= \frac{2}{r_s}\left(2\alpha(x)^2 - 2\alpha(x)\right) \nonumber \\
%   \chi''(r, r_s) &= \frac{4}{r_s^2}\left(4\alpha(x)^3 - 6\alpha(x)^2 + 2\alpha(x)\right) \nonumber \\
%   \chi^{(3)}(r, r_s) &= \frac{8}{r_s^3} \left(12\alpha(x)^4 - 24\alpha(x)^3 + 14\alpha(x)^2 -2 \alpha(x)\right) \nonumber \\
%   \chi^{(4)}(r, r_s) &= \frac{16}{r_s^4} \left(48\alpha(x)^5 - 120\alpha(x)^4 + 100\alpha(x)^3 -30 \alpha(x)^2 + 2\alpha(x)\right) \nonumber \\ 
%   \chi^{(5)}(r, r_s) &= \frac{32}{r_s^5} \left(240\alpha(x)^6 - 720\alpha(x)^5 + 780\alpha(x)^4 - 360\alpha(x)^3 + 62\alpha(x)^2 - 2\alpha(x) \right) \nonumber
% \end{align}


%%%%%%%%%%%%%%%%%%%%%%%%%%%%%%%%%%
\begin{align}
  \mathsf{\tilde{D}}_{1}(r, r_s, H) = % D_tilde_tilde_1 = D_tilde_1 
  \left\lbrace\begin{array}{rcl}
  f(u)\times  H^{-1} & \mbox{if} & u < 1,\\
  %r^{-1} & \mbox{if} & u \geq 1,
  \chi \times r^{-1} & \mbox{if} & u \geq 1~\mbox{and periodic}, \\
  r^{-1} & \mbox{if} & u \geq 1~\mbox{and not periodic}. 
  \end{array}
  \right.\nonumber
\end{align}
%%%%%%%%%%%%%%%%%%%%%%%%%%%%%%%%%%
\begin{align}
  \mathsf{\tilde{D}}_{2}(r, r_s, H) = % D_tilde_tilde_3 = D_tilde_3 * r
  \left\lbrace\begin{array}{rcl}
  f'(u)\times  H^{-2}& \mbox{if} & u < 1,\\
  %-1 \times r^{-3} & \mbox{if} & u \geq 1,
  \left(r\chi' - \chi\right) \times r^{-2} & \mbox{if} & u \geq 1~\mbox{and periodic}, \\
  -1 \times r^{-2} & \mbox{if} & u \geq 1~\mbox{and not periodic}. 
  \end{array}
  \right.\nonumber
\end{align}
%%%%%%%%%%%%%%%%%%%%%%%%%%%%%%%%%%
\begin{align} 
  \mathsf{\tilde{D}}_{3}(r, r_s, H) =  % D_tilde_tilde_5 = D_tilde_5 * r^2
  \left\lbrace\begin{array}{rcl}
  \left(f''(u) - u^{-1}f'(u)\right)\times  H^{-3}& \mbox{if} & u < 1,\\
  %3\times r^{-5} & \mbox{if} & u \geq 1,
  \left(r^2\chi'' - 3r\chi' + 3\chi \right)\times r^{-3} & \mbox{if} & u \geq 1~\mbox{and periodic}, \\
  3 \times  r^{-3} & \mbox{if} & u \geq 1~\mbox{and not periodic}. 
  \end{array}
  \right.\nonumber
\end{align}
%%%%%%%%%%%%%%%%%%%%%%%%%%%%%%%%%%
\begin{align}
  \mathsf{\tilde{D}}_{4}(r, r_s, H) = % D_tilde_tilde_7 = D_tilde_7 * r^3
  \left\lbrace\begin{array}{rcl}
  \left(f^{(3)}(u)-3u^{-1}f''(u)+3u^{-2}f'(u)\right)\times  H^{-4} & \mbox{if} & u < 1,\\
  %-15\times r^{-7} & \mbox{if} & u \geq 1,
  \left(r^3\chi^{(3)} - 6r^2\chi''+15r\chi'-15\chi\right) \times r^{-4} & \mbox{if} & u \geq 1~\mbox{and periodic}, \\
  -15 \times r^{-4} & \mbox{if} & u \geq 1~\mbox{and not periodic}. 
  \end{array}
  \right.\nonumber
\end{align}
%%%%%%%%%%%%%%%%%%%%%%%%%%%%%%%%%%
\begin{align}
  \mathsf{\tilde{D}}_{5}(r, r_s, H) = % D_tilde_tilde_9 = D_tilde_9 * r^4
  \left\lbrace\begin{array}{rcl}
  \left(f^{(4)}(u)-6u^{-1}f^{(3)}(u)+15u^{-2}f''(u)-15u^{-3}f'(u)\right)\times  H^{-5}& \mbox{if} & u < 1,\\
  %105\times r^{-9} & \mbox{if} & u \geq 1.
  \left(r^4\chi^{(4)} - 10r^3\chi^{(3)} + 45r^2\chi'' - 105r\chi' + 105\chi \right) \times r^{-5} & \mbox{if} & u \geq 1~\mbox{and periodic}, \\
  105 \times r^{-5} & \mbox{if} & u \geq 1~\mbox{and not periodic}.
  \end{array}
  \right.\nonumber
\end{align}
%%%%%%%%%%%%%%%%%%%%%%%%%%%%%%%%%%
\begin{align}
  \mathsf{\tilde{D}}_{6}(r, r_s, H) = % D_tilde_tilde_11 = D_tilde_11 * r^4
  \left\lbrace\begin{array}{rcl}
  \left(f^{(5)}(u) -10u^{-1}f^{(4)}(u) +45u^{-2}f^{(3)} -105u^{-3}f''(u) + 105u^{-4}f'(u)\right)\times  H^{-6}& \mbox{if} & u < 1,\\
  %-945\times r^{-11} & \mbox{if} & u \geq 1.
  \left(r^5\chi^{(5)} - 15r^4\chi^{(4)} + 105r^3\chi^{(3)} - 420r^2\chi'' + 945r \chi' - 945\chi\right) \times r^{-6} & \mbox{if} & u \geq 1~\mbox{and periodic}, \\
  -945\times r^{-6} & \mbox{if} & u \geq 1~\mbox{and not periodic}. 
  \end{array}
  \right.\nonumber
\end{align}
In the case $u<1$ and using $f(u)$ given by \ref{eq:fmm:potential}, we can simplify the expressions to get:
\begin{align}
  \mathsf{\tilde{D}}_{1} &= (-3u^7 + 15u^6 - 28u^5 + 21u^4 - 7u^2 + 3) \times H^{-1}, \nonumber \\
  \mathsf{\tilde{D}}_{2} &= (-21u^6 + 90u^5 - 140u^4 + 84u^3 - 14u) \times H^{-2}, \nonumber \\
  \mathsf{\tilde{D}}_{3} &= (-105u^5 + 360u^4 - 420u^3 + 168u^2) \times H^{-3}, \nonumber \\
  \mathsf{\tilde{D}}_{4} &= (-315u^4 + 720u^3 - 420u^2) \times H^{-4}, \nonumber \\
  \mathsf{\tilde{D}}_{5} &= (-315u^3 + 420u) \times H^{-5}, \nonumber \\
  \mathsf{\tilde{D}}_{6} &= (315u^2 - 1260) \times H^{-6}. \nonumber 
\end{align}
We can now write out all the derivatives used in the M2L and M2P kernels:
\begin{align}
  \mathsf{D}_{000}(\mathbf{r}) = \varphi (\mathbf{r}, r_s, H) =
    \mathsf{\tilde{D}}_{1} \nonumber
\end{align}

%%%%%%%%%%%%%%%%%%%%%%%%%%%%%%%%%%
\noindent\rule{6cm}{0.4pt}
\begin{align}
  \mathsf{D}_{100}(\mathbf{r}) = \frac{\partial}{\partial r_x} \varphi (\mathbf{r}, r_s, H) =
    \left(\frac{r_x}{r}\right) \mathsf{\tilde{D}}_{2} \nonumber
\end{align}

%%%%%%%%%%%%%%%%%%%%%%%%%%%%%%%%%%
\noindent\rule{6cm}{0.4pt}
\begin{align}
\mathsf{D}_{200}(\mathbf{r}) = \frac{\partial^2}{\partial r_x^2} \varphi (\mathbf{r}, r_s, H) = 
\left(\frac{r_x}{r}\right)^2 \mathsf{\tilde{D}}_{3} + \left(\frac{1}{r}\right)\mathsf{\tilde{D}}_{2}\nonumber
\end{align}

\begin{align}
\mathsf{D}_{110}(\mathbf{r}) = \frac{\partial^2}{\partial r_x\partial r_y} \varphi (\mathbf{r}, r_s, H) =
\left(\frac{r_x}{r}\right) \left(\frac{r_y}{r}\right)  \mathsf{\tilde{D}}_{3} \nonumber
\end{align}

%%%%%%%%%%%%%%%%%%%%%%%%%%%%%%%%%%
\noindent\rule{6cm}{0.4pt}
\begin{align}
\mathsf{D}_{300}(\mathbf{r}) = \frac{\partial^3}{\partial r_x^3} \varphi (\mathbf{r}, r_s, H) = 
  \left(\frac{r_x}{r}\right)^3 \mathsf{\tilde{D}}_{4}
  + 3 \left(\frac{r_x}{r}\right) \left(\frac{1}{r}\right) \mathsf{\tilde{D}}_{3} \nonumber
\end{align}

\begin{align}
\mathsf{D}_{210}(\mathbf{r}) = \frac{\partial^3}{\partial r_x^2 r_y} \varphi (\mathbf{r}, r_s, H) = 
  \left(\frac{r_x}{r}\right)^2 \left(\frac{r_y}{r}\right) \mathsf{\tilde{D}}_{4} + \left(\frac{r_y}{r}\right) \left(\frac{1}{r}\right) \mathsf{\tilde{D}}_{3} \nonumber
\end{align}

\begin{align}
\mathsf{D}_{111}(\mathbf{r}) = \frac{\partial^3}{\partial r_x\partial r_y\partial r_z} \varphi (\mathbf{r}, r_s, H) = 
\left(\frac{r_x}{r}\right)\left(\frac{r_y}{r}\right)\left(\frac{r_z}{r}\right) \mathsf{\tilde{D}}_{4} \nonumber
\end{align}

%%%%%%%%%%%%%%%%%%%%%%%%%%%%%%%%%%
\noindent\rule{6cm}{0.4pt}
\begin{align}
  \mathsf{D}_{400}(\mathbf{r}) &= \frac{\partial^4}{\partial r_x^4}
  \varphi (\mathbf{r}, r_s, H) =
  \left(\frac{r_x}{r}\right)^4 \mathsf{\tilde{D}}_{5}+
  6\left(\frac{r_x}{r}\right)^2 \left(\frac{1}{r}\right) \mathsf{\tilde{D}}_{4} +
  3 \left(\frac{1}{r}\right)^2 \mathsf{\tilde{D}}_{3}
  \nonumber
\end{align}

\begin{align}
  \mathsf{D}_{310}(\mathbf{r}) &= \frac{\partial^4}{\partial r_x^3
    \partial r_y} \varphi (\mathbf{r}, r_s, H) =
  \left(\frac{r_x}{r}\right)^3 \left(\frac{r_y}{r}\right) \mathsf{\tilde{D}}_{4} +
  3 \left(\frac{r_x}{r}\right) \left(\frac{r_y}{r}\right) \left(\frac{1}{r}\right) \mathsf{\tilde{D}}_{3}
  \nonumber
\end{align}

\begin{align}
  \mathsf{D}_{220}(\mathbf{r}) &= \frac{\partial^4}{\partial r_x^2
    \partial r_y^2} \varphi (\mathbf{r}, r_s, H) =
    \left(\frac{r_x}{r}\right)^2 \left(\frac{r_y}{r}\right)^2 \mathsf{\tilde{D}}_{5} +
    \left(\frac{r_x}{r}\right)^2 \left(\frac{1}{r}\right) \mathsf{\tilde{D}}_{4} +
    \left(\frac{r_y}{r}\right)^2 \left(\frac{1}{r}\right) \mathsf{\tilde{D}}_{4} +
    \left(\frac{1}{r}\right)^2 \mathsf{\tilde{D}}_{3}
  \nonumber
\end{align}

\begin{align}
  \mathsf{D}_{211}(\mathbf{r}) &= \frac{\partial^4}{\partial r_x^2
    \partial r_y   \partial r_z} \varphi (\mathbf{r}, r_s, H) =
    \left(\frac{r_x}{r}\right)^2\left(\frac{r_y}{r}\right)\left(\frac{r_z}{r}\right) \mathsf{\tilde{D}}_{5} +
    \left(\frac{r_y}{r}\right)\left(\frac{r_z}{r}\right)\left(\frac{1}{r}\right) \mathsf{\tilde{D}}_{4}
  \nonumber
\end{align}

%%%%%%%%%%%%%%%%%%%%%%%%%%%%%%%%%%
\noindent\rule{6cm}{0.4pt}
\begin{align}
  \mathsf{D}_{500}(\mathbf{r}) &= \frac{\partial^5}{\partial r_x^5}
  \varphi (\mathbf{r}, r_s, H) =
  \left(\frac{r_x}{r}\right)^5 \mathsf{\tilde{D}}_{6} +
  10\left(\frac{r_x}{r}\right)^3\left(\frac{1}{r}\right)\mathsf{\tilde{D}}_{5} +
  15\left(\frac{r_x}{r}\right)\left(\frac{1}{r}\right)^2\mathsf{\tilde{D}}_{4}
  \nonumber
\end{align}

\begin{align}
  \mathsf{D}_{410}(\mathbf{r}) &= \frac{\partial^5}{\partial r_x^4
    \partial r_y} \varphi (\mathbf{r}, r_s, H) =
  \left(\frac{r_x}{r}\right)^4 \left(\frac{r_y}{r}\right) \mathsf{\tilde{D}}_{6} +
  6 \left(\frac{r_x}{r}\right)^2 \left(\frac{r_y}{r}\right)\left(\frac{1}{r}\right) \mathsf{\tilde{D}}_{5} + 
  3 \left(\frac{r_y}{r}\right) \left(\frac{1}{r}\right)^2\mathsf{\tilde{D}}_{4}
  \nonumber
\end{align}

\begin{align}
  \mathsf{D}_{320}(\mathbf{r}) &= \frac{\partial^5}{\partial r_x^3
    \partial r_y^2} \varphi (\mathbf{r}, r_s, H) =
  \left(\frac{r_x}{r}\right)^3 \left(\frac{r_y}{r}\right)^2 \mathsf{\tilde{D}}_{6} +
  \left(\frac{r_x}{r}\right)^3 \left(\frac{1}{r}\right)\mathsf{\tilde{D}}_{5} +
  3 \left(\frac{r_x}{r}\right) \left(\frac{r_y}{r}\right)^2 \left(\frac{1}{r}\right)\mathsf{\tilde{D}}_{5} + 
  3 \left(\frac{r_x}{r}\right) \left(\frac{1}{r}\right)^2\mathsf{\tilde{D}}_{4}
  \nonumber
\end{align}

\begin{align}
  \mathsf{D}_{311}(\mathbf{r}) &= \frac{\partial^5}{\partial r_x^3
    \partial r_y \partial r_z} \varphi (\mathbf{r}, r_s, H) =
  \left(\frac{r_x}{r}\right)^3 \left(\frac{r_y}{r}\right) \left(\frac{r_z}{r}\right) \mathsf{\tilde{D}}_{6} +
  3 \left(\frac{r_x}{r}\right) \left(\frac{r_y}{r}\right) \left(\frac{r_z}{r}\right) \left(\frac{1}{r}\right)\mathsf{\tilde{D}}_{5}
  \nonumber
\end{align}

\begin{align}
  \mathsf{D}_{221}(\mathbf{r}) &= \frac{\partial^5}{\partial r_x^2
    \partial r_y^2 \partial r_z} \varphi (\mathbf{r}, r_s, H) =
  \left(\frac{r_x}{r}\right)^2 \left(\frac{r_y}{r}\right)^2 \left(\frac{r_z}{r}\right) \mathsf{\tilde{D}}_{6} +
  \left(\frac{r_x}{r}\right)^2 \left(\frac{r_z}{r}\right) \left(\frac{1}{r}\right)\mathsf{\tilde{D}}_{5} +
  \left(\frac{r_y}{r}\right)^2 \left(\frac{r_z}{r}\right) \left(\frac{1}{r}\right)\mathsf{\tilde{D}}_{5} +
  \left(\frac{r_z}{r}\right) \left(\frac{1}{r}\right)^2\mathsf{\tilde{D}}_{4}
  \nonumber
\end{align}

\begin{comment}
\noindent\rule{12cm}{1pt}\\
Old version \\
\noindent\rule{12cm}{1pt}


%%%%%%%%%%%%%%%%%%%%%%%%%%%%%%%%%%
\begin{align}
  \mathsf{\tilde{D}}_{1}(r, r_s, H) =
  \left\lbrace\begin{array}{rcl}
  -\left(3u^7 - 15u^6 + 28u^5 - 21u^4 + 7u^2 - 3\right)\times  H^{-1} & \mbox{if} & u < 1,\\
  %r^{-1} & \mbox{if} & u \geq 1,
  \chi(r, r_s) \times r^{-1} & \mbox{if} & u \geq 1,
  \end{array}
  \right.\nonumber
\end{align}
%%%%%%%%%%%%%%%%%%%%%%%%%%%%%%%%%%
\begin{align}
  \mathsf{\tilde{D}}_{3}(r, r_s, H) =
  \left\lbrace\begin{array}{rcl}
  -\left(21u^5 - 90u^4 + 140u^3 -84u^2 +14\right)\times  H^{-3}& \mbox{if} & u < 1,\\
  %-1 \times r^{-3} & \mbox{if} & u \geq 1,
  \left(r\chi'(r, r_s) - \chi(r, r_s)\right) \times r^{-3} & \mbox{if} & u \geq 1, 
  \end{array}
  \right.\nonumber
\end{align}
%%%%%%%%%%%%%%%%%%%%%%%%%%%%%%%%%%
\begin{align}
  \mathsf{\tilde{D}}_{5}(r, r_s, H) =
  \left\lbrace\begin{array}{rcl}
  -\left(35u^3 - 120u^2 + 140u - 56\right)\times  H^{-5}& \mbox{if} & u < 1,\\
  %3\times r^{-5} & \mbox{if} & u \geq 1,
  \left(r^2\chi''(r, r_s) - 3r\chi'(r, r_s) + 3\chi(r, r_s) \right)\times r^{-5} & \mbox{if} & u \geq 1, 
  \end{array}
  \right.\nonumber
\end{align}
%%%%%%%%%%%%%%%%%%%%%%%%%%%%%%%%%%
\begin{align}
  \mathsf{\tilde{D}}_{7}(r, r_s, H) =
  \left\lbrace\begin{array}{rcl}
  -\left(21u - 48 + 28u^{-1}\right)\times  H^{-7} & \mbox{if} & u < 1,\\
  %-15\times r^{-7} & \mbox{if} & u \geq 1,
  \left(r^3\chi^{(3)}(r, r_s) - 6r^2\chi''(r, r_s)+15r\chi'(r, r_s)-15\chi(r, r_s)\right) \times r^{-7} & \mbox{if} & u \geq 1, 
  \end{array}
  \right.\nonumber
\end{align}
%%%%%%%%%%%%%%%%%%%%%%%%%%%%%%%%%%
\begin{align}
  \mathsf{\tilde{D}}_{9}(r, r_s, H) =
  \left\lbrace\begin{array}{rcl}
  -\left(3u^{-1} - 4u^{-3}\right)\times  H^{-9}& \mbox{if} & u < 1,\\
  %105\times r^{-9} & \mbox{if} & u \geq 1.
  \left(r^4\chi^{(4)}(r, r_s) - 10r^3\chi^{(3)} + 45r^2\chi''(r, r_s) - 105r\chi'(r, r_s) + 105\chi(r, r_s) \right) \times r^{-9} & \mbox{if} & u \geq 1
  \end{array}
  \right.\nonumber
\end{align}
%%%%%%%%%%%%%%%%%%%%%%%%%%%%%%%%%%
\begin{align}
  \mathsf{\tilde{D}}_{11}(r, r_s, H) =
  \left\lbrace\begin{array}{rcl}
  -\left(\frac{1}{3}u^{-3} - \frac{4}{3}u^{-5}\right)\times  H^{-11}& \mbox{if} & u < 1,\\
  %-945\times r^{-11} & \mbox{if} & u \geq 1.
  \left(r^5\chi^{(5)}(r, r_s) - 15r^4\chi^{(4)}(r, r_s) + 105r^3\chi^{(3)}(r, r_s) - 420r^2\chi''(r, r_s) + 945r \chi'(r, r_s) - 945\chi(r, r_s)\right) \times r^{-11} & \mbox{if} & u \geq 1.
  \end{array}
  \right.\nonumber
\end{align}
%%%%%%%%%%%%%%%%%%%%%%%%%%%%%%%%%%
Starting from the potential (Eq. \ref{eq:fmm:potential},
reproduced here for completeness), we can now build all the relevent derivatives
\begin{align}
  \mathsf{D}_{000}(\mathbf{r}) = \varphi (\mathbf{r}, r_s, H) =
    \mathsf{\tilde{D}}_{1}(r, r_s, H) \nonumber
\end{align}

%%%%%%%%%%%%%%%%%%%%%%%%%%%%%%%%%%
\noindent\rule{6cm}{0.4pt}
\begin{align}
  \mathsf{D}_{100}(\mathbf{r}) = \frac{\partial}{\partial r_x} \varphi (\mathbf{r}, r_s, H) =
    r_x \mathsf{\tilde{D}}_{3}(r, r_s, H) \nonumber
\end{align}

%%%%%%%%%%%%%%%%%%%%%%%%%%%%%%%%%%
\noindent\rule{6cm}{0.4pt}
\begin{align}
\mathsf{D}_{200}(\mathbf{r}) = \frac{\partial^2}{\partial r_x^2} \varphi (\mathbf{r}, r_s, H) = 
r_x^2 \mathsf{\tilde{D}}_{5}(r, r_s, H) +
\mathsf{\tilde{D}}_{3}(r, r_s, H)\nonumber
\end{align}

\begin{align}
\mathsf{D}_{110}(\mathbf{r}) = \frac{\partial^2}{\partial r_x\partial r_y} \varphi (\mathbf{r}, r_s, H) = 
   r_x r_y \mathsf{\tilde{D}}_{5}(r, r_s, H) \nonumber
\end{align}

%%%%%%%%%%%%%%%%%%%%%%%%%%%%%%%%%%
\noindent\rule{6cm}{0.4pt}
\begin{align}
\mathsf{D}_{300}(\mathbf{r}) = \frac{\partial^3}{\partial r_x^3} \varphi (\mathbf{r}, r_s, H) = 
  r_x^3 \mathsf{\tilde{D}}_{7}(r, r_s, H)
  + 3 r_x \mathsf{\tilde{D}}_{5}(r, r_s, H) \nonumber
\end{align}

\begin{align}
\mathsf{D}_{210}(\mathbf{r}) = \frac{\partial^3}{\partial r_x^2 r_y} \varphi (\mathbf{r}, r_s, H) = 
r_x^2 r_y \mathsf{\tilde{D}}_{7}(r, r_s, H) +
r_y \mathsf{\tilde{D}}_{5}(r, r_s, H) \nonumber
\end{align}

\begin{align}
\mathsf{D}_{111}(\mathbf{r}) = \frac{\partial^3}{\partial r_x\partial r_y\partial r_z} \varphi (\mathbf{r}, r_s, H) = 
  r_x r_y r_z \mathsf{\tilde{D}}_{7}(r, r_s, H) \nonumber
\end{align}

%%%%%%%%%%%%%%%%%%%%%%%%%%%%%%%%%%
\noindent\rule{6cm}{0.4pt}
\begin{align}
  \mathsf{D}_{400}(\mathbf{r}) &= \frac{\partial^4}{\partial r_x^4}
  \varphi (\mathbf{r}, r_s, H) =
  r_x^4 \mathsf{\tilde{D}}_{9}(r, r_s, H)+
  6r_x^2 \mathsf{\tilde{D}}_{7}(r, r_s, H) +
  3 \mathsf{\tilde{D}}_{5}(r, r_s, H)
  \nonumber
\end{align}

\begin{align}
  \mathsf{D}_{310}(\mathbf{r}) &= \frac{\partial^4}{\partial r_x^3
    \partial r_y} \varphi (\mathbf{r}, r_s, H) =
  r_x^3 r_y \mathsf{\tilde{D}}_{9}(r, r_s, H) +
  3 r_x r_y \mathsf{\tilde{D}}_{7}(r, r_s, H)
  \nonumber
\end{align}

\begin{align}
  \mathsf{D}_{220}(\mathbf{r}) &= \frac{\partial^4}{\partial r_x^2
    \partial r_y^2} \varphi (\mathbf{r}, r_s, H) =
    r_x^2 r_y^2 \mathsf{\tilde{D}}_{9}(r, r_s, H) +
    r_x^2 \mathsf{\tilde{D}}_{7}(r, r_s, H) +
    r_y^2 \mathsf{\tilde{D}}_{7}(r, r_s, H) +
    \mathsf{\tilde{D}}_{5}(r, r_s, H)
  \nonumber
\end{align}

\begin{align}
  \mathsf{D}_{211}(\mathbf{r}) &= \frac{\partial^4}{\partial r_x^2
    \partial r_y   \partial r_z} \varphi (\mathbf{r}, r_s, H) =
    r_x^2 r_y r_z \mathsf{\tilde{D}}_{9}(r, r_s, H) +
    r_y r_z \mathsf{\tilde{D}}_{7}(r, r_s, H)
  \nonumber
\end{align}

%%%%%%%%%%%%%%%%%%%%%%%%%%%%%%%%%%
\noindent\rule{6cm}{0.4pt}
\begin{align}
  \mathsf{D}_{500}(\mathbf{r}) &= \frac{\partial^5}{\partial r_x^5}
  \varphi (\mathbf{r}, r_s, H) =
  r_x^5 \mathsf{\tilde{D}}_{11}(r, r_s, H) +
  10r_x^3\mathsf{\tilde{D}}_{9}(r, r_s, H) +
  15r_x\mathsf{\tilde{D}}_{7}(r, r_s, H)
  \nonumber
\end{align}

\begin{align}
  \mathsf{D}_{410}(\mathbf{r}) &= \frac{\partial^5}{\partial r_x^4
    \partial r_y} \varphi (\mathbf{r}, r_s, H) =
  r_x^4 r_y \mathsf{\tilde{D}}_{11}(r, r_s, H) +
  6 r_x^2 r_y \mathsf{\tilde{D}}_{9}(r, r_s, H) + 
  3 r_y \mathsf{\tilde{D}}_{7}(r, r_s, H)
  \nonumber
\end{align}

\begin{align}
  \mathsf{D}_{320}(\mathbf{r}) &= \frac{\partial^5}{\partial r_x^3
    \partial r_y^2} \varphi (\mathbf{r}, r_s, H) =
  r_x^3 r_y^2 \mathsf{\tilde{D}}_{11}(r, r_s, H) +
  r_x^3 \mathsf{\tilde{D}}_{9}(r, r_s, H) +
  3 r_x r_y^2 \mathsf{\tilde{D}}_{9}(r, r_s, H) + 
  3 r_x \mathsf{\tilde{D}}_{7}(r, r_s, H)
  \nonumber
\end{align}

\begin{align}
  \mathsf{D}_{311}(\mathbf{r}) &= \frac{\partial^5}{\partial r_x^3
    \partial r_y \partial r_z} \varphi (\mathbf{r}, r_s, H) =
  r_x^3 r_y r_z \mathsf{\tilde{D}}_{11}(r, r_s, H) +
  3 r_x r_y r_z \mathsf{\tilde{D}}_{9}(r, r_s, H)
  \nonumber
\end{align}

\begin{align}
  \mathsf{D}_{221}(\mathbf{r}) &= \frac{\partial^5}{\partial r_x^2
    \partial r_y^2 \partial r_z} \varphi (\mathbf{r}, r_s, H) =
  r_x^2 r_y^2 r_z \mathsf{\tilde{D}}_{11}(r, r_s, H) +
  r_x^2 r_z \mathsf{\tilde{D}}_{9}(r, r_s, H) +
  r_y^2 r_z \mathsf{\tilde{D}}_{9}(r, r_s, H) +
  r_z \mathsf{\tilde{D}}_{7}(r, r_s, H)
  \nonumber
\end{align}

\end{comment}



















